Add definition rules

theories/stlc_types.v
@@ -1,5 +1,6 @@
-Require Export tactics rlist.
 From Ltac2 Require Export Rewrite.
+From stdpp Require Export relations.
+Require Export tactics rlist.
 
 
 (*********************************************)
@@ -72,54 +73,60 @@ Module TyTheories (Ty : TY).
   Ltac2 Notation "ty_simpl" "in" h(ident) := ty_simpl (one_hyp h).
   Ltac2 Notation "ty_simpl" := ty_simpl goal.
   (* Tactic Notation "ty_simpl" "in" "*" := repeat (simpl in *; autorewrite with ty in * ).  *)
-  Ltac2 Notation "ty_induction" h(constr) := induction $h using ty_rect.
+  Ltac2 Notation "ty_induction" h(ident) :=
+    Control.enter (fun () =>
+      let c := Control.hyp h in induction $c using ty_rect
+    ).
 
 
   (** *** View *)
 
-  Module ty_view.
-    Inductive tyv : Set :=
-      | tyv_prp : tyv
-      | tyv_arr : tyv -> tyv -> tyv
-      | tyv_other : ty -> tyv.
+  Inductive tyv : Set :=
+    | tyv_prp : tyv
+    | tyv_arr : tyv -> tyv -> tyv
+    | tyv_other : ty -> tyv.
 
-    Definition to_tyv : ty -> tyv :=
-      ty_rec _
-        tyv_prp
-        (fun _ fA _ fB => tyv_arr fA fB)
-        (fun T _ => tyv_other T).
+  Definition to_tyv : ty -> tyv :=
+    ty_rec _
+      tyv_prp
+      (fun _ fA _ fB => tyv_arr fA fB)
+      (fun T _ => tyv_other T).
 
-    Theorem to_tyv_prp : to_tyv ty_prp = tyv_prp.
-    Proof. unfold to_tyv. now ty_simpl. Qed.
+  Theorem to_tyv_prp : to_tyv ty_prp = tyv_prp.
+  Proof. unfold to_tyv. now ty_simpl. Qed.
 
-    Theorem to_tyv_arr A B :
-      to_tyv (ty_arr A B) = tyv_arr (to_tyv A) (to_tyv B).
-    Proof.
-      unfold to_tyv. now ty_simpl.
-    Qed.
+  Theorem to_tyv_arr A B :
+    to_tyv (ty_arr A B) = tyv_arr (to_tyv A) (to_tyv B).
+  Proof.
+    unfold to_tyv. now ty_simpl.
+  Qed.
 
-    Theorem to_tyv_other T : ty_other T ->
-      to_tyv T = tyv_other T.
-    Proof.
-      intros. unfold to_tyv. now ty_simpl.
-    Qed.
+  Theorem to_tyv_other T : ty_other T ->
+    to_tyv T = tyv_other T.
+  Proof.
+    intros. unfold to_tyv. now ty_simpl.
+  Qed.
 
 
-    Fixpoint to_ty T : ty :=
-      match T with
-      | tyv_prp => ty_prp
-      | tyv_arr A B => ty_arr (to_ty A) (to_ty B)
-      | tyv_other T => T
-      end.
+  Fixpoint to_ty T : ty :=
+    match T with
+    | tyv_prp => ty_prp
+    | tyv_arr A B => ty_arr (to_ty A) (to_ty B)
+    | tyv_other T => T
+    end.
 
-    Theorem to_ty_to_tyv T : to_ty (to_tyv T) = T.
-    Proof.
-      ty_induction T.
-      - now rewrite to_tyv_prp.
-      - rewrite to_tyv_arr. simpl. congruence.
-      - now rewrite to_tyv_other.
-    Qed.
-  End ty_view.
+  Theorem to_ty_to_tyv T : to_ty (to_tyv T) = T.
+  Proof.
+    ty_induction T.
+    - now rewrite to_tyv_prp.
+    - rewrite to_tyv_arr. simpl. congruence.
+    - now rewrite to_tyv_other.
+  Qed.
+
+  Create HintDb tyv.
+  Hint Rewrite to_tyv_arr : tyv.
+  Ltac2 tyv_simpl c := autorewrite @tyv c; s_simpl c.
+  Ltac2 Notation "tyv_simpl" := tyv_simpl goal.
 
 
   (** *** Injection and discriminate *)
@@ -127,10 +134,10 @@ Module TyTheories (Ty : TY).
   Theorem ty_arr_inj {X Y A B} : ty_arr X Y = ty_arr A B -> X = A /\ Y = B.
   Proof.
     intros H.
-    apply (f_equal ty_view.to_tyv) in H. repeat (rewrite ty_view.to_tyv_arr in H).
+    apply (f_equal to_tyv) in H. repeat (rewrite to_tyv_arr in H).
     injection H. intros HY HX.
-    apply (f_equal ty_view.to_ty) in HY. apply (f_equal ty_view.to_ty) in HX.
-    repeat (rewrite ty_view.to_ty_to_tyv in *). auto.
+    apply (f_equal to_ty) in HY. apply (f_equal to_ty) in HX.
+    repeat (rewrite to_ty_to_tyv in *). auto.
   Qed.
 
   Ltac2 Notation "ty_injection" h(ident) :=
@@ -174,6 +181,44 @@ Module TyTheories (Ty : TY).
     - destruct (IHx1 y1), (IHx2 y2); subst; try (now left);
         right; intros N; ty_injection N; congruence.
     - now apply ty_eq_dec_other.
+  Qed.
+
+
+  Definition ty_size T : nat :=
+    (fix fx T :=
+      match T with
+      | tyv_arr A B => fx A + fx B + 1
+      | _ => 0
+    end) (to_tyv T).
+
+  Theorem ty_size_arr X Y : ty_size -[ X -> Y ]- = ty_size X + ty_size Y + 1.
+  Proof. unfold ty_size. now tyv_simpl. Qed.
+
+  Definition ty_sub_b X Y := exists Z, Y = -[ X -> Z ]- \/ Y = -[ Z -> X ]-.
+  Definition ty_sub := tc ty_sub_b.
+
+  Theorem ty_sub_size X Y : ty_sub X Y -> ty_size X < ty_size Y.
+  Proof.
+    intros H.
+    induction H; destruct H as [Z [HZ | HZ]]; subst; rewrite ty_size_arr in *; lia.
+  Qed.
+
+  Instance ty_sub_order : StrictOrder ty_sub.
+  Proof.
+    constructor.
+    - intros x Hx.
+      apply ty_sub_size in Hx. lia.
+    - apply tc_transitive.
+  Qed.
+
+  Theorem ty_sub_foldr T L : L <> [] -> ty_sub T (foldr ty_arr T L).
+  Proof.
+    intros HL. induction L > [congruence|].
+    simpl. destruct L as [|L]; simpl in *.
+    - constructor. exists a. now right.
+    - etransitivity.
+      + apply IHL. discriminate.
+      + constructor. exists a. now right.
   Qed.
 
 
