theories/glogic.v
@@ -39,489 +39,693 @@ Module tm_set : TM_SET.
   Qed.
 End tm_set.
 
-Export tm_set.
+
+Module Type CLAUSES.
+  Parameter clause_f : list ty -> nat -> option gtm.
+  Axiom clause_f_spec : forall C l n B, clause_f l n = Some B ->
+    let T := type_check_other (gtm_prd l n) in
+    has_type C B (ty_arr T T).
+End CLAUSES.
 
 
-Notation is_form C t := (has_type C t ty_prp).
-Definition wf_tm_set C (l : tm_set) := forall t, t ∈ l -> is_form C t.
-
-Definition wf_sequent C (p : tm_set) c := wf_tm_set C p /\ is_form C c.
-
-Instance wf_sequent_Proper : Proper ((=) ==> (≡) ==> (=) ==> iff) wf_sequent.
-Proof.
-  intros C ? <- p q E c ? <-.
-  unfold wf_sequent, wf_tm_set. intuition; set_solver.
-Qed.
+Module GLogic.
+  Declare Module Clauses : CLAUSES.
+  Export tm_set.
+  Export Clauses.
 
 
-(***********************)
-(** ** Deduction rules *)
-(***********************)
+  Notation is_form C t := (has_type C t ty_prp).
+  Definition wf_tm_set C (l : tm_set) := forall t, t ∈ l -> is_form C t.
 
-Notation "∅" := empty (in custom stlc_ty) : stlc_scope.
-Notation "∅" := empty (in custom stlc_tm) : stlc_scope.
-Notation "∅" := empty : stdpp_scope.
-Infix "∪" := union (in custom stlc_tm at level 50) : stlc_scope.
-Infix "∪" := union : stdpp_scope.
-Notation "s +; x" := (s ∪ {[x]}) (in custom stlc_tm at level 50, left associativity) : stlc_scope.
-Notation "s +; x" := (s ∪ {[x]}) (at level 50, left associativity) : stlc_scope.
-Notation "{[ x ]}" := (singleton x) (in custom stlc_tm) : stlc_scope.
-Notation "{[ x ]}" := (singleton x) : stdpp_scope.
+  Definition wf_sequent C (p : tm_set) c := wf_tm_set C p /\ is_form C c.
 
+  Instance wf_sequent_Proper : Proper ((=) ==> (≡) ==> (=) ==> iff) wf_sequent.
+  Proof.
+    intros C ? <- p q E c ? <-.
+    unfold wf_sequent, wf_tm_set. intuition; set_solver.
+  Qed.
 
-Inductive is_derivable_wf : context -> tm_set -> tm -> Prop :=
-  | wrl_set C l m c :
-      l ≡ m ->
-      is_derivable_wf C l c ->
-      is_derivable_wf C m c
-  | wrl_id C a b :
-      has_type C a ty_prp ->
-      has_type C b ty_prp ->
-      tm_equiv C a b ->
-      is_derivable_wf C {[a]} b
-  | wrl_cut C l m b c :
-      is_derivable_wf C l b ->
-      is_derivable_wf C (m +; b) c ->
-      is_derivable_wf C (l ∪ m) c
-  | wrl_cL C l b c :
-      is_derivable_wf C (l +; b +; b) c ->
-      is_derivable_wf C (l +; b) c
-  | wrl_wL C l m b :
-      (forall a, a ∈ l -> has_type C a ty_prp) ->
-      is_derivable_wf C m b ->
-      is_derivable_wf C (l ∪ m) b
-  | wrl_botL C c :
-      has_type C c ty_prp ->
-      is_derivable_wf C {[gtm_bot]} c
-  | wrl_topR C :
-      is_derivable_wf C ∅ gtm_top
-  | wrl_orL C l b c d :
-      is_derivable_wf C (l +; b) c ->
-      is_derivable_wf C (l +; d) c ->
-      is_derivable_wf C (l +; <{ b \/ d }>) c
-  | wrl_orR1 C l b c :
-      has_type C c ty_prp ->
-      is_derivable_wf C l b ->
-      is_derivable_wf C l <{ b \/ c }>
-  | wrl_orR2 C l b c :
-      has_type C b ty_prp ->
-      is_derivable_wf C l c ->
-      is_derivable_wf C l <{ b \/ c }>
-  | wrl_andL1 C l b c d :
-      has_type C d ty_prp ->
-      is_derivable_wf C (l +; b) c ->
-      is_derivable_wf C (l +; <{ b /\ d }>) c
-  | wrl_andL2 C l b c d :
-      has_type C b ty_prp ->
-      is_derivable_wf C (l +; d) c ->
-      is_derivable_wf C (l +; <{ b /\ d }>) c
-  | wrl_andR C l b c :
-      is_derivable_wf C l b ->
-      is_derivable_wf C l c ->
-      is_derivable_wf C l <{ b /\ c }>
-  | wrl_impL C l b c d :
-      is_derivable_wf C l b ->
-      is_derivable_wf C (l +; d) c ->
-      is_derivable_wf C (l +; <{ b > d }>) c
-  | wrl_impR C l b c :
-      is_derivable_wf C (l +; b) c ->
-      is_derivable_wf C l <{ b > c }>
-  | wrl_forL C T l b c t :
-      has_type C t T ->
-      is_derivable_wf C (l +; subst_last C C t b) c ->
-      is_derivable_wf C (l +; <{for T, b}>) c
-  | wrl_forR C T l b sb :
-      (forall t, t ∈ sb <-> in_supp b t) ->
-      is_derivable_wf (C +: foldr ty_arr T (type_check_other <$> sb)) (tm_set_map (lift C) l) (
-        subst_last C (S C) (foldl tm_app (tm_lvl C) sb) b
-      ) ->
-      is_derivable_wf C l <{for T, b}>
-  | wrl_exL C T l b c sb :
-      (forall t, t ∈ sb <-> in_supp b t) ->
-      is_derivable_wf (C +: foldr ty_arr T (type_check_other <$> sb)) (
-        tm_set_map (lift C) l ∪
-        {[subst_last C (S C) (foldl tm_app (tm_lvl C) sb) b]}
-      ) (lift C c) ->
-      is_derivable_wf C (l +; <{ex T, b}>) c
-  | wrl_exR C T l b t :
-      has_type C t T ->
-      is_derivable_wf C l (subst_last C C t b) ->
-      is_derivable_wf C l <{ex T, b}>
-  | wrl_nabL {T b} n (_ : ~ in_supp b (gtm_nom T n)) C l c :
-    is_derivable_wf C (l +; subst_last C C (gtm_nom T n) b) c ->
-    is_derivable_wf C (l +; <{nab T, b}>) c
-  | wrl_nabR {T b} n (_ : ~ in_supp b (gtm_nom T n)) C l :
-      is_derivable_wf C l (subst_last C C (gtm_nom T n) b) ->
-      is_derivable_wf C l (<{nab T, b}>)
-.
+  (***************)
+  (** ** Clauses *)
+  (***************)
 
-Inductive is_derivable : context -> tm_set -> tm -> Prop :=
-  | rl_set C l m c :
-      l ≡ m ->
-      is_derivable C l c ->
-      is_derivable C m c
-  | rl_id (C : context) l a b :
-      tm_equiv C a b ->
-      is_derivable C (l +; a) b
-  | rl_cut C l m b c :
-      has_type C b ty_prp ->
-      is_derivable C l b ->
-      is_derivable C (m +; b) c ->
-      is_derivable C (l ∪ m) c
-  | rl_cL C l b c :
-      is_derivable C (l +; b +; b) c ->
-      is_derivable C (l +; b) c
-  | rl_botL C l c :
-      is_derivable C (l +; gtm_bot) c
-  | rl_topR C l :
-      is_derivable C l gtm_top
-  | rl_orL C l b c d :
-      is_derivable C (l +; b) c ->
-      is_derivable C (l +; d) c ->
-      is_derivable C (l +; <{ b \/ d }>) c
-  | rl_orR1 C l b c :
-      is_derivable C l b ->
-      is_derivable C l <{ b \/ c }>
-  | rl_orR2 C l b c :
-      is_derivable C l c ->
-      is_derivable C l <{ b \/ c }>
-  | rl_andL1 C l b c d :
-      is_derivable C (l +; b) c ->
-      is_derivable C (l +; <{ b /\ d }>) c
-  | rl_andL2 C l b c d :
-      is_derivable C (l +; d) c ->
-      is_derivable C (l +; <{ b /\ d }>) c
-  | rl_andR C l b c :
-      is_derivable C l b ->
-      is_derivable C l c ->
-      is_derivable C l <{ b /\ c }>
-  | rl_impL C l b c d :
-      is_derivable C l b ->
-      is_derivable C (l +; d) c ->
-      is_derivable C (l +; <{ b > d }>) c
-  | rl_impR C l b c :
-      is_derivable C (l +; b) c ->
-      is_derivable C l <{ b > c }>
-  | rl_forL C T l b c t :
-      has_type C t T ->
-      is_derivable C (l +; subst_last C C t b) c ->
-      is_derivable C (l +; <{for T, b}>) c
-  | rl_forR C T l b sb :
-      (forall t, t ∈ sb <-> in_supp b t) ->
-      is_derivable (C +: foldr ty_arr T (type_check_other <$> sb)) (tm_set_map (lift C) l) (
-        subst_last C (S C) (foldl tm_app (tm_lvl C) sb) b
-      ) ->
-      is_derivable C l <{for T, b}>
-  | rl_exL C T l b c sb :
-      (forall t, t ∈ sb <-> in_supp b t) ->
-      is_derivable (C +: foldr ty_arr T (type_check_other <$> sb)) (
-        tm_set_map (lift C) l ∪
-        {[subst_last C (S C) (foldl tm_app (tm_lvl C) sb) b]}
-      ) (lift C c) ->
-      is_derivable C (l +; <{ex T, b}>) c
-  | rl_exR C T l b t :
-      has_type C t T ->
-      is_derivable C l (subst_last C C t b) ->
-      is_derivable C l <{ex T, b}>
-  | rl_nabL {T b} n (_ : ~ in_supp b (gtm_nom T n)) C l c :
-  is_derivable C (l +; subst_last C C (gtm_nom T n) b) c ->
-  is_derivable C (l +; <{nab T, b}>) c
-  | rl_nabR {T b} n (_ : ~ in_supp b (gtm_nom T n)) C l :
-      is_derivable C l (subst_last C C (gtm_nom T n) b) ->
-      is_derivable C l (<{nab T, b}>)
-.
+  Theorem has_type_clause {L n B C T} :
+    clause_f L n = Some B ->
+    has_type C B T <->
+    let X := type_check_other (gtm_prd L n) in
+    T = ty_arr X X.
+  Proof.
+    split; intros.
+    - eapply has_type_unique > [eassumption|].
+      now apply clause_f_spec.
+    - simpl in *. subst. eapply clause_f_spec. eassumption.
+  Qed.
 
-Notation "[{ sig ; l --> B }]" := (is_derivable sig l B)
-  (sig custom stlc_ty, l custom stlc_tm, B custom stlc_tm) : stlc_scope.
+  Ltac2 ht_clause h :=
+    let c := Control.hyp h in
+    match! goal with
+    | [ o : clause_f _ _ = Some _ |- _ ] =>
+      let oc := Control.hyp o in let a := Fresh.in_goal @H in
+        assert ($a := proj1 (has_type_clause $oc) $c); simpl in $a; try (ty_injection $a); []
+    end.
+
+  Ltac2 Set ht_list as old := fun () => List.append (old ()) [ht_clause].
+
+  Ltac2 htg_clause () :=
+    match! goal with
+    | [ o : clause_f _ _ = Some _ |- _ ] =>
+        let oc := Control.hyp o in
+        refine '(proj2 (has_type_clause $oc) _); try reflexivity
+    end.
+
+  Ltac2 Set htg_list as old := fun () => List.append (old ()) [htg_clause].
 
 
-Instance is_derivable_wf_Proper :
-  Proper ((=) ==> (≡) ==> (=) ==> iff) is_derivable_wf.
-Proof.
-  intros ? ** ? ** ? **. subst.
-  split; intros H; eapply wrl_set; try (apply H); easy.
-Qed.
+  (***********************)
+  (** ** Deduction rules *)
+  (***********************)
 
-Instance is_derivable_Proper :
-  Proper ((=) ==> (≡) ==> (=) ==> iff) is_derivable.
-Proof.
-  intros ? ** ? ** ? **. subst.
-  split; intros H; eapply rl_set; try (apply H); easy.
-Qed.
-
-
-Theorem has_type_fold C T h l t :
-  Forall2 (fun x X => has_type C x X) l h ->
-  has_type C t (foldr ty_arr T h) ->
-  has_type C (foldl tm_app t l) T.
-Proof.
-  revert h t. induction l; intros h t F Ht.
-  - inversion F. now subst.
-  - simpl. destruct h; inversion F. subst.
-    eapply IHl; try eassumption.
-    has_type. now (exists t0).
-Qed.
-
-Theorem has_type_fold2 C T sb b :
-  (forall t, t ∈ sb -> in_supp b t) ->
-  has_type (C +: foldr ty_arr T (type_check_other <$> sb)) (subst_last C (S C) (foldl tm_app (tm_lvl C) sb) b) -[ o ]- ->
-  has_type (C +: T) b ty_prp.
-Proof.
-  intros.
-  eapply (has_type_subst_last2 _ (C +: foldr ty_arr T (type_check_other <$> sb)));
-    simpl; try eassumption; try lia.
-  - intros. now rewrite decide_True.
-  - eapply has_type_fold; has_type.
-    2:{ simpl. rewrite decide_False; ltac1:(intuition lia). }
-    remember (C +: foldr ty_arr T (type_check_other <$> sb)) as D eqn : ED.
-    clear ED H0. induction sb; simpl in *; constructor.
-    + constructor. set_unfold. eapply in_supp_other. auto.
-    + set_unfold. auto.
-Qed.
-
-Theorem has_type_fold2_2 C T sb b :
-  (forall t, t ∈ sb -> in_supp b t) ->
-  has_type (C +: T) b ty_prp ->
-  has_type (C +: foldr ty_arr T (type_check_other <$> sb)) (subst_last C (S C) (foldl tm_app (tm_lvl C) sb) b) -[ o ]-.
-Proof.
-  intros.
-  eapply has_type_subst_last1.
-  - tm_simpl. lia.
-  - intros. tm_simpl. now rewrite decide_True.
-  - eapply has_type_fold; has_type.
-    2:{ simpl. rewrite decide_False; ltac1:(intuition lia). }
-    remember (C +: foldr ty_arr T (type_check_other <$> sb)) as D eqn : ED.
-    clear ED H0. induction sb; simpl in *; constructor.
-    + constructor. set_unfold. eapply in_supp_other. auto.
-    + set_unfold. auto.
-  - assumption.
-Qed.
-
-Theorem is_derivable_wf_wf C l c : is_derivable_wf C l c -> wf_sequent C l c.
-Proof.
-  intros D. unfold wf_sequent. induction D; simpl in *.
-  - set_unfold. intuition. apply H0. now apply H.
-  - split; try assumption.
-    intros. set_unfold. congruence.
-  - set_unfold. intuition.
-  - set_unfold. intuition.
-  - set_unfold. intuition.
-  - set_unfold. intuition. subst. now constructor.
-  - set_unfold. intuition. now constructor.
-  - set_unfold. intuition. subst.
-    repeat (eapply ht_app); auto. now apply ht_other2.
-  - intuition. repeat (eapply ht_app); try eassumption. now apply ht_other2.
-  - intuition. repeat (eapply ht_app); try eassumption. now apply ht_other2.
-  - set_unfold. intuition. subst.
-    repeat (eapply ht_app); eauto. now apply ht_other2.
-  - set_unfold. intuition. subst.
-    repeat (eapply ht_app); eauto. now apply ht_other2.
-  - intuition. repeat (eapply ht_app); try eassumption. now apply ht_other2.
-  - set_unfold. intuition. subst.
-    repeat (eapply ht_app); eauto. now apply ht_other2.
-  - set_unfold. intuition.
-    repeat (eapply ht_app); eauto. now apply ht_other2.
-  - set_unfold. intuition. subst. econstructor.
-    + now apply ht_other2.
-    + has_type. eapply has_type_subst_last2; eauto.
-  - unfold wf_tm_set. intuition > [|econstructor].
-    + eapply has_type_lift2.
-      apply H0. apply tm_set_map_spec. eauto.
-    + now apply ht_other2.
-    + has_type. eapply has_type_fold2; try eassumption. apply H.
-  - set_unfold. intuition.
-    + eapply has_type_lift2. apply H0. left.
-      apply tm_set_map_spec. eauto.
-    + subst. econstructor > [now apply ht_other2|].
-      has_type. eapply has_type_fold2; auto. apply H.
-    + eapply has_type_lift2; eassumption.
-  - intuition. econstructor > [now apply ht_other2|].
-    has_type. eapply has_type_subst_last2; eauto.
-  - set_unfold. intuition. subst.
-    econstructor > [now apply ht_other2|].
-    has_type. eapply has_type_subst_last2; eauto.
-    now constructor.
-  - intuition. econstructor > [now apply ht_other2|].
-    has_type. eapply has_type_subst_last2; eauto.
-    now constructor.
-Qed.
-
-Theorem rl_wL C l m c :
-  [{ C; m --> c }] -> [{ C; l ∪ m --> c }].
-Proof.
-  revert C l m c.
-  assert (MU : forall C h l, tm_set_map (lift C) <{ h ∪ l }> ≡ (tm_set_map (lift C) h) ∪ (tm_set_map (lift C) l) ). {
-    intros C h1 h2 x. set_unfold. repeat (rewrite tm_set_map_spec).
-    set_unfold. split.
-    - intros [y [Hy ->]]. destruct Hy; ltac1:(intuition eauto).
-    - intros [[y [Hy ->]] | [y [Hy ->]]]; eauto.
-  }
-  intros * H. revert l.
-  induction H; intros h; try (rewrite union_assoc in *).
-  - now rewrite <- H.
-  - now apply rl_id.
-  - eapply rl_cut; eauto.
-  - apply rl_cL. specialize IHis_derivable with h.
-    now repeat (rewrite union_assoc in *).
-  - apply rl_botL.
-  - apply rl_topR.
-  - apply rl_orL; now rewrite <- union_assoc.
-  - now apply rl_orR1.
-  - now apply rl_orR2.
-  - apply rl_andL1; now rewrite <- union_assoc.
-  - apply rl_andL2; now rewrite <- union_assoc.
-  - now apply rl_andR.
-  - apply rl_impL > [easy|]. now rewrite <- union_assoc.
-  - apply rl_impR. now rewrite <- union_assoc.
-  - eapply rl_forL > [eassumption|].
-    now rewrite <- union_assoc.
-  - eapply rl_forR; try eassumption.
-    now rewrite MU.
-  - eapply rl_exL; try eassumption.
-    now rewrite MU, <- union_assoc.
-  - eapply rl_exR; eauto.
-  - eapply rl_nabL; try eassumption.
-    now rewrite <- union_assoc.
-  - eapply rl_nabR; eauto.
-Qed.
-
-Theorem is_derivable_wf_is_derivable C l c :
-  is_derivable_wf C l c -> [{ C; l --> c }].
-Proof.
-  intros DW. induction DW; subst.
-  - eapply rl_set; eassumption.
-  - rewrite <- union_empty. now apply rl_id.
-  - eapply rl_cut; try eassumption.
-    apply is_derivable_wf_wf in DW1. destruct DW1. assumption.
-  - now apply rl_cL.
-  - now apply rl_wL.
-  - rewrite <- union_empty. apply rl_botL.
-  - apply rl_topR.
-  - now apply rl_orL.
-  - now apply rl_orR1.
-  - now apply rl_orR2.
-  - now apply rl_andL1.
-  - now apply rl_andL2.
-  - now apply rl_andR.
-  - now apply rl_impL.
-  - now apply rl_impR.
-  - eapply rl_forL; eassumption.
-  - eapply rl_forR; eassumption.
-  - eapply rl_exL; eassumption.
-  - eapply rl_exR; eassumption.
-  - eapply rl_nabL; eassumption.
-  - eapply rl_nabR; eassumption.
-Qed.
-
-Theorem is_derivable_is_derivable_wf C l c :
-  wf_sequent C l c ->  [{ C; l --> c }] -> is_derivable_wf C l c.
-Proof.
-  intros [] D. unfold wf_tm_set in *. induction D; set_unfold.
-  - eapply wrl_set > [eassumption|].
-    apply IHD; set_solver.
-  - apply wrl_wL; try auto.
-    apply wrl_id; auto.
-  - eapply wrl_cut; first [apply IHD1 | apply IHD2]; set_solver.
-  - apply wrl_cL. apply IHD; set_solver.
-  - apply wrl_wL > [|apply wrl_botL]; set_solver.
-  - assert (E : l ≡ l ∪ ∅) > [set_solver|].
-    rewrite E. apply wrl_wL > [|apply wrl_topR].
-    clear E. set_solver.
-  - assert (is_form C <{b \/ d}>) by auto.
-    apply wrl_orL; first [apply IHD1 | apply IHD2];
-      intuition; subst; now has_type.
-  - apply wrl_orR1.
-    + now has_type.
-    + apply IHD; intuition. now has_type.
-  - apply wrl_orR2.
-    + now has_type.
-    + apply IHD; intuition. now has_type.
-  - assert (is_form C <{b /\ d}>) by auto.
-    apply wrl_andL1 > [now has_type|].
-    apply IHD; intuition. subst. now has_type.
-  - assert (is_form C <{b /\ d}>) by auto.
-    apply wrl_andL2 > [now has_type|].
-    apply IHD; intuition. subst. now has_type.
-  - assert (is_form C <{b /\ c}>) by auto. apply wrl_andR.
-    + apply IHD1. intuition. now has_type.
-    + apply IHD2. intuition. now has_type.
-  - assert (is_form C <{b > d}>) by auto. apply wrl_impL.
-    + apply IHD1. intuition. now has_type.
-    + apply IHD2; intuition. subst. now has_type.
-  - assert (is_form C <{b > c}>) by auto. apply wrl_impR.
-    apply IHD; intuition; subst; now has_type.
-  - eapply wrl_forL > [eassumption|].
-    apply IHD; intuition. subst.
-    eapply has_type_subst_last_s1 > [eassumption|].
-    assert (is_form C <{for T, b}>) by auto.
-    now has_type.
-  - eapply wrl_forR > [eassumption|].
-    apply IHD; intuition.
-    + apply tm_set_map_spec in H2 as [a [Ha1 Ha2]]. subst.
-      has_type. auto.
-    + apply has_type_fold2_2 > [apply H1|].
-      now has_type.
-  - eapply wrl_exL > [eassumption|].
-    apply IHD; intuition.
-    + apply tm_set_map_spec in H3 as [a [Ha1 Ha2]]. subst.
-      has_type. auto.
-    + subst. apply has_type_fold2_2 > [apply H1|].
-      assert (is_form C <{ex T, b}>) by auto.
-      now has_type.
-    + now has_type.
-  - eapply wrl_exR > [eassumption|].
-    apply IHD; intuition.
-    eapply has_type_subst_last_s1 > [eassumption|].
-    now has_type.
-  - eapply wrl_nabL > [eassumption|].
-    apply IHD; intuition. subst.
-    eapply has_type_subst_last_s1.
-    + now apply ht_other.
-    + assert (is_form C <{nab T, b}>) by auto.
-      now has_type.
-  - eapply wrl_nabR > [eassumption|].
-    apply IHD; intuition.
-    eapply has_type_subst_last_s1.
-    + now apply ht_other.
-    + now has_type.
-Qed.
+  Notation "∅" := empty (in custom stlc_ty) : stlc_scope.
+  Notation "∅" := empty (in custom stlc_tm) : stlc_scope.
+  Notation "∅" := empty : stdpp_scope.
+  Infix "∪" := union (in custom stlc_tm at level 50) : stlc_scope.
+  Infix "∪" := union : stdpp_scope.
+  Notation "s +; x" := (s ∪ {[x]}) (in custom stlc_tm at level 50, left associativity) : stlc_scope.
+  Notation "s +; x" := (s ∪ {[x]}) (at level 50, left associativity) : stlc_scope.
+  Notation "{[ x ]}" := (singleton x) (in custom stlc_tm) : stlc_scope.
+  Notation "{[ x ]}" := (singleton x) : stdpp_scope.
 
 
-Theorem rl_nabL2 C T b l c :
-  exists2 n, ~ in_supp b (gtm_nom T n) &
-  (is_derivable C (l ∪ {[ subst_last C C (gtm_nom T n) b ]}) c ->
-  is_derivable C (l ∪ {[ <{nab T, b}> ]}) c).
-Proof.
-  exists (nom_fresh b).
-  - apply nom_fresh_in_supp.
-  - intros. eapply rl_nabL.
-    + apply nom_fresh_in_supp.
-    + eassumption.
-Qed.
+  Inductive is_derivable_wf : context -> tm_set -> tm -> Prop :=
+    | wrl_set C l m c :
+        l ≡ m ->
+        is_derivable_wf C l c ->
+        is_derivable_wf C m c
+    | wrl_id C a b :
+        has_type C a ty_prp ->
+        has_type C b ty_prp ->
+        tm_equiv C a b ->
+        is_derivable_wf C {[a]} b
+    | wrl_cut C l m b c :
+        is_derivable_wf C l b ->
+        is_derivable_wf C (m +; b) c ->
+        is_derivable_wf C (l ∪ m) c
+    | wrl_cL C l b c :
+        is_derivable_wf C (l +; b +; b) c ->
+        is_derivable_wf C (l +; b) c
+    | wrl_wL C l m b :
+        (forall a, a ∈ l -> has_type C a ty_prp) ->
+        is_derivable_wf C m b ->
+        is_derivable_wf C (l ∪ m) b
+    | wrl_botL C c :
+        has_type C c ty_prp ->
+        is_derivable_wf C {[gtm_bot]} c
+    | wrl_topR C :
+        is_derivable_wf C ∅ gtm_top
+    | wrl_orL C l b c d :
+        is_derivable_wf C (l +; b) c ->
+        is_derivable_wf C (l +; d) c ->
+        is_derivable_wf C (l +; <{ b \/ d }>) c
+    | wrl_orR1 C l b c :
+        has_type C c ty_prp ->
+        is_derivable_wf C l b ->
+        is_derivable_wf C l <{ b \/ c }>
+    | wrl_orR2 C l b c :
+        has_type C b ty_prp ->
+        is_derivable_wf C l c ->
+        is_derivable_wf C l <{ b \/ c }>
+    | wrl_andL1 C l b c d :
+        has_type C d ty_prp ->
+        is_derivable_wf C (l +; b) c ->
+        is_derivable_wf C (l +; <{ b /\ d }>) c
+    | wrl_andL2 C l b c d :
+        has_type C b ty_prp ->
+        is_derivable_wf C (l +; d) c ->
+        is_derivable_wf C (l +; <{ b /\ d }>) c
+    | wrl_andR C l b c :
+        is_derivable_wf C l b ->
+        is_derivable_wf C l c ->
+        is_derivable_wf C l <{ b /\ c }>
+    | wrl_impL C l b c d :
+        is_derivable_wf C l b ->
+        is_derivable_wf C (l +; d) c ->
+        is_derivable_wf C (l +; <{ b > d }>) c
+    | wrl_impR C l b c :
+        is_derivable_wf C (l +; b) c ->
+        is_derivable_wf C l <{ b > c }>
+    | wrl_forL C T l b c t :
+        has_type C t T ->
+        is_derivable_wf C (l +; subst_last C C t b) c ->
+        is_derivable_wf C (l +; <{for T, b}>) c
+    | wrl_forR C T l b sb :
+        (forall t, t ∈ sb <-> in_supp b t) ->
+        is_derivable_wf (C +: foldr ty_arr T (type_check_other <$> sb)) (tm_set_map (lift C) l) (
+          subst_last C (S C) (foldl tm_app (tm_lvl C) sb) b
+        ) ->
+        is_derivable_wf C l <{for T, b}>
+    | wrl_exL C T l b c sb :
+        (forall t, t ∈ sb <-> in_supp b t) ->
+        is_derivable_wf (C +: foldr ty_arr T (type_check_other <$> sb)) (
+          tm_set_map (lift C) l ∪
+          {[subst_last C (S C) (foldl tm_app (tm_lvl C) sb) b]}
+        ) (lift C c) ->
+        is_derivable_wf C (l +; <{ex T, b}>) c
+    | wrl_exR C T l b t :
+        has_type C t T ->
+        is_derivable_wf C l (subst_last C C t b) ->
+        is_derivable_wf C l <{ex T, b}>
+    | wrl_nabL {T b} n (_ : ~ in_supp b (gtm_nom T n)) C l c :
+        is_derivable_wf C (l +; subst_last C C (gtm_nom T n) b) c ->
+        is_derivable_wf C (l +; <{nab T, b}>) c
+    | wrl_nabR {T b} n (_ : ~ in_supp b (gtm_nom T n)) C l :
+        is_derivable_wf C l (subst_last C C (gtm_nom T n) b) ->
+        is_derivable_wf C l (<{nab T, b}>)
+    | wrl_defL C l L n B c t :
+        let p := gtm_prd L n in
+        clause_f L n = Some B ->
+        is_derivable_wf C (l +; foldl tm_app <{B p}> t) c ->
+        is_derivable_wf C (l +; foldl tm_app p t) c
+    | wrl_defR C l L n B t :
+        let p := gtm_prd L n in
+        clause_f L n = Some B ->
+        is_derivable_wf C l (foldl tm_app <{B p}> t) ->
+        is_derivable_wf C l (foldl tm_app p t)
+  .
 
-(*
-Ltac rl_nabL n := edestruct rl_nabL2 as [n ?X ?H]; apply H; clear H.
-*)
+  Inductive is_derivable : context -> tm_set -> tm -> Prop :=
+    | rl_set C l m c :
+        l ≡ m ->
+        is_derivable C l c ->
+        is_derivable C m c
+    | rl_id (C : context) l a b :
+        tm_equiv C a b ->
+        is_derivable C (l +; a) b
+    | rl_cut C l m b c :
+        has_type C b ty_prp ->
+        is_derivable C l b ->
+        is_derivable C (m +; b) c ->
+        is_derivable C (l ∪ m) c
+    | rl_cL C l b c :
+        is_derivable C (l +; b +; b) c ->
+        is_derivable C (l +; b) c
+    | rl_botL C l c :
+        is_derivable C (l +; gtm_bot) c
+    | rl_topR C l :
+        is_derivable C l gtm_top
+    | rl_orL C l b c d :
+        is_derivable C (l +; b) c ->
+        is_derivable C (l +; d) c ->
+        is_derivable C (l +; <{ b \/ d }>) c
+    | rl_orR1 C l b c :
+        is_derivable C l b ->
+        is_derivable C l <{ b \/ c }>
+    | rl_orR2 C l b c :
+        is_derivable C l c ->
+        is_derivable C l <{ b \/ c }>
+    | rl_andL1 C l b c d :
+        is_derivable C (l +; b) c ->
+        is_derivable C (l +; <{ b /\ d }>) c
+    | rl_andL2 C l b c d :
+        is_derivable C (l +; d) c ->
+        is_derivable C (l +; <{ b /\ d }>) c
+    | rl_andR C l b c :
+        is_derivable C l b ->
+        is_derivable C l c ->
+        is_derivable C l <{ b /\ c }>
+    | rl_impL C l b c d :
+        is_derivable C l b ->
+        is_derivable C (l +; d) c ->
+        is_derivable C (l +; <{ b > d }>) c
+    | rl_impR C l b c :
+        is_derivable C (l +; b) c ->
+        is_derivable C l <{ b > c }>
+    | rl_forL C T l b c t :
+        has_type C t T ->
+        is_derivable C (l +; subst_last C C t b) c ->
+        is_derivable C (l +; <{for T, b}>) c
+    | rl_forR C T l b sb :
+        (forall t, t ∈ sb <-> in_supp b t) ->
+        is_derivable (C +: foldr ty_arr T (type_check_other <$> sb)) (tm_set_map (lift C) l) (
+          subst_last C (S C) (foldl tm_app (tm_lvl C) sb) b
+        ) ->
+        is_derivable C l <{for T, b}>
+    | rl_exL C T l b c sb :
+        (forall t, t ∈ sb <-> in_supp b t) ->
+        is_derivable (C +: foldr ty_arr T (type_check_other <$> sb)) (
+          tm_set_map (lift C) l ∪
+          {[subst_last C (S C) (foldl tm_app (tm_lvl C) sb) b]}
+        ) (lift C c) ->
+        is_derivable C (l +; <{ex T, b}>) c
+    | rl_exR C T l b t :
+        has_type C t T ->
+        is_derivable C l (subst_last C C t b) ->
+        is_derivable C l <{ex T, b}>
+    | rl_nabL {T b} n (_ : ~ in_supp b (gtm_nom T n)) C l c :
+    is_derivable C (l +; subst_last C C (gtm_nom T n) b) c ->
+    is_derivable C (l +; <{nab T, b}>) c
+    | rl_nabR {T b} n (_ : ~ in_supp b (gtm_nom T n)) C l :
+        is_derivable C l (subst_last C C (gtm_nom T n) b) ->
+        is_derivable C l (<{nab T, b}>)
+    | rl_defL C l L n B c t :
+        let p := gtm_prd L n in
+        clause_f L n = Some B ->
+        is_derivable C (l +; foldl tm_app <{B p}> t) c ->
+        is_derivable C (l +; foldl tm_app p t) c
+    | rl_defR C l L n B t :
+        let p := gtm_prd L n in
+        clause_f L n = Some B ->
+        is_derivable C l (foldl tm_app <{B p}> t) ->
+        is_derivable C l (foldl tm_app p t)
+  .
 
-Theorem tm_set_swap (l : tm_set) a b :
-  <{ l +; a +; b }> ≡ <{ l +; b +; a }>.
-Proof. set_unfold. intuition. Qed.
+  Notation "[{ sig ; l --> B }]" := (is_derivable sig l B)
+    (sig custom stlc_ty, l custom stlc_tm, B custom stlc_tm) : stlc_scope.
 
-Theorem contrapositive C l b c :
-  [{ C ; l +; b --> c }] -> [{ C ; l +; ~ c --> ~ b }].
-Proof.
-  intros H.
-  apply rl_impR. rewrite tm_set_swap.
-  apply rl_impL; try assumption.
-  apply rl_botL.
-Qed.
 
-Hint Rewrite in_supp_not : tm.
+  Instance is_derivable_wf_Proper :
+    Proper ((=) ==> (≡) ==> (=) ==> iff) is_derivable_wf.
+  Proof.
+    intros ? ** ? ** ? **. subst.
+    split; intros H; eapply wrl_set; try (apply H); easy.
+  Qed.
 
-Theorem rl_id2 C l t : is_derivable C (l ∪ {[t]}) t.
-Proof. intros. apply rl_id; easy. Qed.
+  Instance is_derivable_Proper :
+    Proper ((=) ==> (≡) ==> (=) ==> iff) is_derivable.
+  Proof.
+    intros ? ** ? ** ? **. subst.
+    split; intros H; eapply rl_set; try (apply H); easy.
+  Qed.
 
-(*
-Notation "({ C ; l --> c })" := (wf_sequent C l c -> is_derivable C l c)
-  (C custom stlc_ty, l custom stlc_tm, c custom stlc_tm) : stlc_scope.
+
+  (*
+  Theorem has_type_fold C T A h l t :
+    length h = length l ->
+    has_type C t (foldr ty_arr T h) ->
+    has_type C (foldl tm_app t l) A ->
+    A = T.
+  Proof.
+    intros L H1 H2.
+    apply has_type_fold_app in H2 as [X H2 F].
+    apply (has_type_unique _ _ H1) in H2.
+    clear l t L H1 F.
+  Qed.
   *)
+
+  (*
+  Theorem has_type_fold C T h l t :
+    has_type C t (foldr ty_arr T h) ->
+    Forall2 (fun x X => has_type C x X) l h ->
+    has_type C (foldl tm_app t l) T.
+  Proof.
+    revert h t. induction l; intros h t Ht F.
+    - inversion F. now subst.
+    - simpl. destruct h; inversion F. subst.
+      eapply IHl; try eassumption.
+      has_type. now (exists t0).
+  Qed.
+
+  Theorem th T l :
+    l <> [] -> T <> foldr ty_arr T l.
+  Proof.
+    intros Hl E. destruct l > [congruence|]. simpl in *.
+    clear Hl. revert t l E.
+    ty_induction T; intros t l E; try (ty_discriminate E).
+    rewrite <- foldr_snoc in E.
+    destruct l.
+    - simpl in *. ty_injection E.
+      clear IHT1 IHT2 E E0.
+      ty_induction T2; try (ty_discriminate E1).
+      ty_injection E1. auto.
+    - simpl in E. ty_injection E.
+      eapply IHT2. rewrite <- E1.
+      eassumption.
+  Qed.
+
+  Theorem th2 C T t l :
+    l <> [] ->
+    has_type C (foldl tm_app t l) T -> has_type C t T -> False.
+  Proof.
+    revert t. induction l > [congruence|]; intros t Hl H1 H2.
+    simpl in *. eapply IHl.
+    2:{ eassumption. }
+    2:{ has_type.
+
+  Theorem has_type_fold_2 C T h l t :
+    has_type C t (foldr ty_arr T h) ->
+    has_type C (foldl tm_app t l) T ->
+    Forall2 (fun x X => has_type C x X) l h.
+  Proof.
+    revert t h. induction l; intros t h Ht H.
+    - simpl in *.
+      apply (has_type_unique _ _ H) in Ht.
+      clear H. destruct h > [constructor|].
+      apply th in Ht > [easy|].
+      congruence.
+    - destruct h.
+      + simpl in *.
+        Search foldl.
+        rewrite <- foldl_snoc in H.
+        has_type.
+      simpl in *. clear IHh. exfalso.
+      ty_induction T; try (ty_discriminate Ht).
+      destruct h; simpl in *.
+      + ty_injection Ht. auto.
+      + simpl in Ht.
+        ty_injection Ht.
+        apply IHT2.
+        assert (forall A B l, foldr ty_arr (ty_arr A B) l = ty_arr (foldr ty_arr A l) B). {
+          intros. induction l; simpl in *; try reflexivity.
+          rewrite IHl. simpl.
+          -
+        }
+  - (* Case ty_arr T1 T2 *)
+    destruct l as [| a l']; [congruence |].
+    simpl in Ht. ltac1:(ty_injection Ht).
+    (* H1 is the equality for the codomain: T2 = foldr ty_arr (ty_arr T1 T2) l' *)
+    rewrite foldr_ty_arr_append in H1.
+    eapply (H0 (l' ++ [T1])); [|assumption].
+    intros N. ltac1:(apply app_eq_nil in N as [_ N]; discriminate).
+  - (* Case ty_other *)
+    destruct l; [congruence | simpl in Ht; ltac1:(ty_discriminate Ht)].exfalso.
+      revert T Ht.
+      induction h; intros T Ht.
+      + simpl in Ht.
+        ty_induction T; try (ty_discriminate Ht).
+        ty_injection Ht. auto.
+      + simpl in *.
+        ty_induction T; try (ty_discriminate Ht).
+        eapply IHh. apply Ht.
+      + constructor.
+      + simpl in *.
+  Admitted.
+  *)
+
+  Theorem has_type_fold C T sb b :
+    (forall t, t ∈ sb -> in_supp b t) ->
+    has_type (C +: foldr ty_arr T (type_check_other <$> sb)) (subst_last C (S C) (foldl tm_app (tm_lvl C) sb) b) -[ o ]- ->
+    has_type (C +: T) b ty_prp.
+  Proof.
+    intros.
+    eapply (has_type_subst_last2 _ (C +: foldr ty_arr T (type_check_other <$> sb)));
+      simpl; try eassumption; try lia.
+    - intros. now rewrite decide_True.
+    - apply has_type_fold_app. eexists; has_type.
+      + simpl. rewrite decide_False; ltac1:(intuition lia).
+      + remember (C +: foldr ty_arr T (type_check_other <$> sb)) as D eqn : ED.
+        clear ED H0. induction sb; simpl in *; constructor.
+        * constructor. set_unfold. eapply in_supp_other. auto.
+        * set_unfold. auto.
+  Qed.
+
+  Theorem has_type_fold2 C T sb b :
+    (forall t, t ∈ sb -> in_supp b t) ->
+    has_type (C +: T) b ty_prp ->
+    has_type (C +: foldr ty_arr T (type_check_other <$> sb)) (subst_last C (S C) (foldl tm_app (tm_lvl C) sb) b) -[ o ]-.
+  Proof.
+    intros.
+    eapply has_type_subst_last1.
+    - simpl. lia.
+    - intros. simpl. now rewrite decide_True.
+    - apply has_type_fold_app. eexists; has_type.
+      + simpl. rewrite decide_False; ltac1:(intuition lia).
+      + remember (C +: foldr ty_arr T (type_check_other <$> sb)) as D eqn : ED.
+        clear ED H0. induction sb; simpl in *; constructor.
+        * constructor. set_unfold. eapply in_supp_other. auto.
+        * set_unfold. auto.
+    - assumption.
+  Qed.
+
+  Theorem foldr_ty_arr_inj T L M :
+    foldr ty_arr T L = foldr ty_arr T M -> L = M.
+  Proof.
+    revert M.
+    induction L; intros M E. simpl in *.
+    - destruct (decide (M = [])) > [easy|].
+      exfalso. apply (StrictOrder_Irreflexive T).
+      rewrite E at 2. now apply ty_sub_foldr.
+    - destruct M; simpl in *.
+      + rewrite <- foldr_cons in E.
+        exfalso. apply (StrictOrder_Irreflexive T).
+        rewrite <- E at 2. now apply ty_sub_foldr.
+      + ty_injection E. f_equal. now apply IHL.
+  Qed.
+
+  Theorem is_derivable_wf_wf C l c : is_derivable_wf C l c -> wf_sequent C l c.
+  Proof.
+    intros D. unfold wf_sequent. induction D; simpl in *.
+    - set_unfold. intuition. apply H0. now apply H.
+    - split; try assumption.
+      intros. set_unfold. congruence.
+    - set_unfold. intuition.
+    - set_unfold. intuition.
+    - set_unfold. intuition.
+    - set_unfold. intuition. subst. now constructor.
+    - set_unfold. intuition. now constructor.
+    - set_unfold. intuition. subst.
+      repeat (eapply ht_app); auto. now apply ht_other2.
+    - intuition. repeat (eapply ht_app); try eassumption. now apply ht_other2.
+    - intuition. repeat (eapply ht_app); try eassumption. now apply ht_other2.
+    - set_unfold. intuition. subst.
+      repeat (eapply ht_app); eauto. now apply ht_other2.
+    - set_unfold. intuition. subst.
+      repeat (eapply ht_app); eauto. now apply ht_other2.
+    - intuition. repeat (eapply ht_app); try eassumption. now apply ht_other2.
+    - set_unfold. intuition. subst.
+      repeat (eapply ht_app); eauto. now apply ht_other2.
+    - set_unfold. intuition.
+      repeat (eapply ht_app); eauto. now apply ht_other2.
+    - set_unfold. intuition. subst. econstructor.
+      + now apply ht_other2.
+      + has_type. eapply has_type_subst_last2; eauto.
+    - unfold wf_tm_set. intuition > [|econstructor].
+      + eapply has_type_lift2.
+        apply H0. apply tm_set_map_spec. eauto.
+      + now apply ht_other2.
+      + has_type. eapply has_type_fold; try eassumption. apply H.
+    - set_unfold. intuition.
+      + eapply has_type_lift2. apply H0. left.
+        apply tm_set_map_spec. eauto.
+      + subst. econstructor > [now apply ht_other2|].
+        has_type. eapply has_type_fold; auto. apply H.
+      + eapply has_type_lift2; eassumption.
+    - intuition. econstructor > [now apply ht_other2|].
+      has_type. eapply has_type_subst_last2; eauto.
+    - set_unfold. intuition. subst.
+      econstructor > [now apply ht_other2|].
+      has_type. eapply has_type_subst_last2; eauto.
+      now constructor.
+    - intuition. econstructor > [now apply ht_other2|].
+      has_type. eapply has_type_subst_last2; eauto.
+      now constructor.
+    - set_unfold. intuition. subst.
+      assert (is_form C (foldl tm_app <{ B p }> t)) by auto.
+      has_type.
+      exists L > [assumption|].
+      ltac1:(replace L with x) > [assumption|].
+      eapply foldr_ty_arr_inj. eassumption.
+    - set_unfold. intuition.
+      has_type. exists L > [assumption|].
+      ltac1:(replace L with x) > [assumption|].
+      eapply foldr_ty_arr_inj. eassumption.
+  Qed.
+
+  Theorem rl_wL C l m c :
+    [{ C; m --> c }] -> [{ C; l ∪ m --> c }].
+  Proof.
+    revert C l m c.
+    assert (MU : forall C h l, tm_set_map (lift C) <{ h ∪ l }> ≡ (tm_set_map (lift C) h) ∪ (tm_set_map (lift C) l) ). {
+      intros C h1 h2 x. set_unfold. repeat (rewrite tm_set_map_spec).
+      set_unfold. split.
+      - intros [y [Hy ->]]. destruct Hy; ltac1:(intuition eauto).
+      - intros [[y [Hy ->]] | [y [Hy ->]]]; eauto.
+    }
+    intros * H. revert l.
+    induction H; intros h; try (rewrite union_assoc in *).
+    - now rewrite <- H.
+    - now apply rl_id.
+    - eapply rl_cut; eauto.
+    - apply rl_cL. specialize IHis_derivable with h.
+      now repeat (rewrite union_assoc in *).
+    - apply rl_botL.
+    - apply rl_topR.
+    - apply rl_orL; now rewrite <- union_assoc.
+    - now apply rl_orR1.
+    - now apply rl_orR2.
+    - apply rl_andL1; now rewrite <- union_assoc.
+    - apply rl_andL2; now rewrite <- union_assoc.
+    - now apply rl_andR.
+    - apply rl_impL > [easy|]. now rewrite <- union_assoc.
+    - apply rl_impR. now rewrite <- union_assoc.
+    - eapply rl_forL > [eassumption|].
+      now rewrite <- union_assoc.
+    - eapply rl_forR; try eassumption.
+      now rewrite MU.
+    - eapply rl_exL; try eassumption.
+      now rewrite MU, <- union_assoc.
+    - eapply rl_exR; eauto.
+    - eapply rl_nabL; try eassumption.
+      now rewrite <- union_assoc.
+    - eapply rl_nabR; eauto.
+    - eapply rl_defL > [eassumption|].
+      now rewrite <- union_assoc.
+    - eapply rl_defR; eauto.
+  Qed.
+
+  Theorem is_derivable_wf_is_derivable C l c :
+    is_derivable_wf C l c -> [{ C; l --> c }].
+  Proof.
+    intros DW. induction DW; subst.
+    - eapply rl_set; eassumption.
+    - rewrite <- union_empty. now apply rl_id.
+    - eapply rl_cut; try eassumption.
+      apply is_derivable_wf_wf in DW1. destruct DW1. assumption.
+    - now apply rl_cL.
+    - now apply rl_wL.
+    - rewrite <- union_empty. apply rl_botL.
+    - apply rl_topR.
+    - now apply rl_orL.
+    - now apply rl_orR1.
+    - now apply rl_orR2.
+    - now apply rl_andL1.
+    - now apply rl_andL2.
+    - now apply rl_andR.
+    - now apply rl_impL.
+    - now apply rl_impR.
+    - eapply rl_forL; eassumption.
+    - eapply rl_forR; eassumption.
+    - eapply rl_exL; eassumption.
+    - eapply rl_exR; eassumption.
+    - eapply rl_nabL; eassumption.
+    - eapply rl_nabR; eassumption.
+    - eapply rl_defL; eassumption.
+    - eapply rl_defR; eassumption.
+  Qed.
+
+  Theorem is_derivable_is_derivable_wf C l c :
+    wf_sequent C l c ->  [{ C; l --> c }] -> is_derivable_wf C l c.
+  Proof.
+    intros [] D. unfold wf_tm_set in *. induction D; set_unfold.
+    - eapply wrl_set > [eassumption|].
+      apply IHD; set_solver.
+    - apply wrl_wL; try auto.
+      apply wrl_id; auto.
+    - eapply wrl_cut; first [apply IHD1 | apply IHD2]; set_solver.
+    - apply wrl_cL. apply IHD; set_solver.
+    - apply wrl_wL > [|apply wrl_botL]; set_solver.
+    - assert (E : l ≡ l ∪ ∅) > [set_solver|].
+      rewrite E. apply wrl_wL > [|apply wrl_topR].
+      clear E. set_solver.
+    - assert (is_form C <{b \/ d}>) by auto.
+      apply wrl_orL; first [apply IHD1 | apply IHD2];
+        intuition; subst; now has_type.
+    - apply wrl_orR1.
+      + now has_type.
+      + apply IHD; intuition. now has_type.
+    - apply wrl_orR2.
+      + now has_type.
+      + apply IHD; intuition. now has_type.
+    - assert (is_form C <{b /\ d}>) by auto.
+      apply wrl_andL1 > [now has_type|].
+      apply IHD; intuition. subst. now has_type.
+    - assert (is_form C <{b /\ d}>) by auto.
+      apply wrl_andL2 > [now has_type|].
+      apply IHD; intuition. subst. now has_type.
+    - assert (is_form C <{b /\ c}>) by auto. apply wrl_andR.
+      + apply IHD1. intuition. now has_type.
+      + apply IHD2. intuition. now has_type.
+    - assert (is_form C <{b > d}>) by auto. apply wrl_impL.
+      + apply IHD1. intuition. now has_type.
+      + apply IHD2; intuition. subst. now has_type.
+    - assert (is_form C <{b > c}>) by auto. apply wrl_impR.
+      apply IHD; intuition; subst; now has_type.
+    - eapply wrl_forL > [eassumption|].
+      apply IHD; intuition. subst.
+      eapply has_type_subst_last_s1 > [eassumption|].
+      assert (is_form C <{for T, b}>) by auto.
+      now has_type.
+    - eapply wrl_forR > [eassumption|].
+      apply IHD; intuition.
+      + apply tm_set_map_spec in H2 as [a [Ha1 Ha2]]. subst.
+        has_type. auto.
+      + apply has_type_fold2 > [apply H1|].
+        now has_type.
+    - eapply wrl_exL > [eassumption|].
+      apply IHD; intuition.
+      + apply tm_set_map_spec in H3 as [a [Ha1 Ha2]]. subst.
+        has_type. auto.
+      + subst. apply has_type_fold2 > [apply H1|].
+        assert (is_form C <{ex T, b}>) by auto.
+        now has_type.
+      + now has_type.
+    - eapply wrl_exR > [eassumption|].
+      apply IHD; intuition.
+      eapply has_type_subst_last_s1 > [eassumption|].
+      now has_type.
+    - eapply wrl_nabL > [eassumption|].
+      apply IHD; intuition. subst.
+      eapply has_type_subst_last_s1.
+      + now apply ht_other.
+      + assert (is_form C <{nab T, b}>) by auto.
+        now has_type.
+    - eapply wrl_nabR > [eassumption|].
+      apply IHD; intuition.
+      eapply has_type_subst_last_s1.
+      + now apply ht_other.
+      + now has_type.
+    - eapply wrl_defL > [eassumption|].
+      apply IHD; intuition. subst.
+      assert (is_form C (foldl tm_app p t)) by auto.
+      has_type. exists L.
+      + has_type_goal (). eexists > [|eassumption].
+        has_type_goal ().
+      + ltac1:(replace L with x) > [assumption|].
+        eapply foldr_ty_arr_inj. eassumption.
+    - eapply wrl_defR > [eassumption|].
+      apply IHD; intuition.
+      has_type. exists L.
+      + has_type_goal (). eexists > [|eassumption].
+        has_type_goal ().
+      + ltac1:(replace L with x) > [assumption|].
+        eapply foldr_ty_arr_inj. eassumption.
+  Qed.
+
+
+  Theorem rl_nabL2 C T b l c :
+    exists2 n, ~ in_supp b (gtm_nom T n) &
+    (is_derivable C (l ∪ {[ subst_last C C (gtm_nom T n) b ]}) c ->
+    is_derivable C (l ∪ {[ <{nab T, b}> ]}) c).
+  Proof.
+    exists (nom_fresh b).
+    - apply nom_fresh_in_supp.
+    - intros. eapply rl_nabL.
+      + apply nom_fresh_in_supp.
+      + eassumption.
+  Qed.
+
+  (*
+  Ltac rl_nabL n := edestruct rl_nabL2 as [n ?X ?H]; apply H; clear H.
+  *)
+
+  Theorem tm_set_swap (l : tm_set) a b :
+    <{ l +; a +; b }> ≡ <{ l +; b +; a }>.
+  Proof. set_unfold. intuition. Qed.
+
+  Theorem contrapositive C l b c :
+    [{ C ; l +; b --> c }] -> [{ C ; l +; ~ c --> ~ b }].
+  Proof.
+    intros H.
+    apply rl_impR. rewrite tm_set_swap.
+    apply rl_impL; try assumption.
+    apply rl_botL.
+  Qed.
+
+  Hint Rewrite in_supp_not : tm.
+
+  Theorem rl_id2 C l t : is_derivable C (l ∪ {[t]}) t.
+  Proof. intros. apply rl_id; easy. Qed.
+
+  (*
+  Notation "({ C ; l --> c })" := (wf_sequent C l c -> is_derivable C l c)
+    (C custom stlc_ty, l custom stlc_tm, c custom stlc_tm) : stlc_scope.
+    *)
+End GLogic.
